work on getting lock for disk_idx

examples/scache/Cache.i.dfy
@@ -1,23 +1,32 @@
 include "AtomicRefcount.i.dfy"
 include "AtomicStatus.i.dfy"
+include "AtomicIndexLookup.i.dfy"
+include "ArrayPtr.s.dfy"
 
 module CacheImpl {
   import opened Constants
   import opened AtomicStatusImpl
   import opened AtomicRefcountImpl
-  import opened Ptrs
+  import opened AtomicIndexLookupImpl
   import opened LinearMaybe
+  import opened Ptrs
+  import opened NativeTypes
+  import opened Options
 
   datatype Cache = Cache(
     data: seq<Ptr>,
+    disk_idx_of_entry: seq<Ptr>,
+
     status: seq<AtomicStatus>,
     read_refcounts: seq<seq<AtomicRefcount>>,
-    disk_idx_lookup: seq<AtomicIndexLookup>
+
+    cache_idx_of_page: seq<AtomicIndexLookup>
   )
 
   predicate Inv(c: Cache)
   {
     && |c.data| == CacheSize()
+    && |c.disk_idx_of_entry| == CacheSize()
     && |c.status| == CacheSize()
     && (forall i | 0 <= i < CacheSize() ::
        atomic_status_inv(c.status[i], c.data[i]))
@@ -26,14 +35,40 @@ module CacheImpl {
         |c.read_refcounts[j]| == CacheSize())
     && (forall j, i | 0 <= j < NThreads() && 0 <= i < CacheSize() ::
         atomic_refcount_inv(c.read_refcounts[j][i], c.data[i], j))
+    && |c.cache_idx_of_page| == NDiskPages()
     && (forall d | 0 <= d < NDiskPages() ::
-        |c.disk_idx_lookup| == NDiskPages())
+        atomic_index_lookup_inv(c.cache_idx_of_page[d], d))
+  }
+
+  linear datatype CacheEntryHandle = CacheEntryHandle(
+      linear cache_entry: CacheResources.R,
+      linear data: ArrayDeref<byte>,
+      linear idx: Deref<int>
+  )
+  {
+    predicate is_handle(c: Cache, cache_idx: int)
+    requires Inv(c)
+    {
+      && 0 <= cache_idx < CacheSize()
+      && data.ptr == c.data[cache_idx]
+      && idx.ptr == c.disk_idx_of_entry[cache_idx]
+      && cache_entry == CacheResources.CacheEntry(Some(idx.v), cache_idx, data.s)
+    }
+
+    predicate is_page_handle(c: Cache, disk_idx: int)
+    requires Inv(c)
+    {
+      && cache_entry.CacheEntry?
+      && is_handle(c, cache_entry.cache_idx)
+      && cache_entry.disk_idx_opt == Some(disk_idx)
+    }
   }
 
   method take_write_lock_on_cache_entry(c: Cache, cache_idx: int)
-  returns (linear w: ReadWriteLockResources.Q)
+  returns (linear handle: CacheEntryHandle)
   requires Inv(c)
   requires 0 <= cache_idx < CacheSize()
+  ensures handle.is_handle(c, cache_idx)
   decreases *
   {
     linear var w_maybe := empty();
@@ -50,6 +85,7 @@ module CacheImpl {
           c.status[cache_idx], c.data[cache_idx]);
     }
 
+    linear var w;
     w := unwrap(w_maybe);
 
     success := false;
@@ -86,11 +122,53 @@ module CacheImpl {
 
       j := j + 1;
     }
+
+    // TODO
+    handle := AtomicRefcountImpl.unsafe_obtain();
+    AtomicRefcountImpl.unsafe_dispose(w);
+    assume false;
   }
+
+  method release_write_lock_on_cache_entry(c: Cache, cache_idx: int,
+      linear handle: CacheEntryHandle)
+  requires Inv(c)
+  requires 0 <= cache_idx < CacheSize()
+  requires handle.is_handle(c, cache_idx)
 
   /*method take_write_lock_on_disk_entry(c: Cache, disk_idx: int)
   requires 0 
   {
     
   }*/
+
+  method try_take_write_lock_disk_page(c: Cache, disk_idx: int)
+  returns (success: bool, linear handle_out: maybe<CacheEntryHandle>)
+  requires Inv(c)
+  requires 0 <= disk_idx < NDiskPages()
+  ensures !success ==> handle_out == empty()
+  ensures success ==> has(handle_out) &&
+      peek(handle_out).is_page_handle(c, disk_idx)
+  decreases *
+  {
+    var cache_idx := atomic_index_lookup_read(c.cache_idx_of_page[disk_idx], disk_idx);
+
+    if cache_idx == NOT_MAPPED {
+      // TODO
+      success := false;
+      handle_out := empty();
+    } else {
+      linear var handle := take_write_lock_on_cache_entry(c, cache_idx as int);
+      var this_disk_idx := ptr_read(
+          c.disk_idx_of_entry[cache_idx],
+          handle.idx);
+      if this_disk_idx == disk_idx {
+        success := true;
+        handle_out := give(handle);
+      } else {
+        release_write_lock_on_cache_entry(c, cache_idx as int, handle);
+        success := false;
+        handle_out := empty();
+      }
+    }
+  }
 }
